{
  "@context": {
    "@version": 1.1,
    "dct": "http://purl.org/dc/terms/",
    "owl": "http://www.w3.org/2002/07/owl#",
    "rdf": "http://www.w3.org/1999/02/22-rdf-syntax-ns#",
    "rdfa": "http://www.w3.org/ns/rdfa#",
    "rdfs": "http://www.w3.org/2000/01/rdf-schema#",
    "schema": "http://schema.org/",
    "xsd": "http://www.w3.org/2001/XMLSchema#",
    "skos": "http://www.w3.org/2004/02/skos/core#",
    "prov": "http://www.w3.org/ns/prov#",
    "pav": "http://purl.org/pav/",
    "nidm": "http://purl.org/nidash/nidm#",
    "uuid": "http://uuid.repronim.org/",
    "reproschema": "http://schema.repronim.org/"
  },
  "@graph": [
    {
      "@id": "reproschema:AllowExport",
      "@type": "rdfs:Class",
      "rdfs:comment": "Indicates (by boolean) if data can be exported or not.",
      "rdfs:label": "Allow export"
    },
    {
      "@id": "reproschema:multipleChoice",
      "@type": "rdf:Property",
      "schema:rangeIncludes": {
        "@id": "schema:Boolean"
      },
      "rdfs:comment": "Indicates (by bool) if response for the Field item has one or more answer.",
      "rdfs:label": "Multiple choice response expectation"
    },
    {
      "@id": "reproschema:order",
      "@type": "rdf:Property",
      "schema:rangeIncludes": [
        {
          "@id": "reproschema:Activity"
        },
        {
          "@id": "reproschema:Field"
        },
        {
          "@id": "schema:URL"
        }
      ],
      "rdfs:comment": "An ordered list to describe the order in which the items of an assessment or protocol appear in the user interface.",
      "rdfs:label": "Order"
    },
    {
      "@id": "reproschema:inputType",
      "@type": "rdf:Property",
      "schema:rangeIncludes": {
        "@id": "schema:Text"
      },
      "rdfs:comment": "An element to describe the input type of a Field item.",
      "rdfs:label": "inputType"
    },
    {
      "@id": "reproschema:maxRetakes",
      "@type": "rdf:Property",
      "schema:rangeIncludes": {
        "@id": "schema:Number"
      },
      "rdfs:comment": "Defines number of times the item is allowed to be redone.",
      "rdfs:label": "maxRetakes"
    },
    {
      "@id": "reproschema:AllowReplay",
      "@type": "rdfs:Class",
      "rdfs:comment": "Indicates (by boolean) if items can be replayed or not.",
      "rdfs:label": "Allow replay"
    },
    {
      "@id": "reproschema:schedule",
      "@type": "rdf:Property",
      "schema:rangeIncludes": [
        {
          "@id": "schema:Text"
        },
        {
          "@id": "schema:Schedule"
        }
      ],
      "rdfs:comment": "An element to set make activity available/repeat info using ISO 8601 repeating interval format.",
      "rdfs:label": "Schedule"
    },
    {
      "@id": "reproschema:shuffle",
      "@type": "rdf:Property",
      "schema:rangeIncludes": {
        "@id": "schema:boolean"
      },
      "rdfs:comment": "An element (bool) to determine if the list of items is shuffled or in order.",
      "rdfs:label": "Shuffle"
    },
    {
      "@id": "reproschema:DontKnow",
      "@type": "rdfs:Class",
      "rdfs:comment": "An element to describe the choice when response is not known.",
      "rdfs:label": "Do not know"
    },
    {
      "@id": "reproschema:isAbout",
      "schema:domainIncludes": {
        "@id": "reproschema:Response"
      }
    },
    {
      "@id": "schema:value",
      "schema:domainIncludes": {
        "@id": "reproschema:Response"
      },
      "schema:rangeIncludes": [
        {
          "@id": "reproschema:Skipped"
        },
        {
          "@id": "reproschema:DontKnow"
        },
        {
          "@id": "schema:Number"
        },
        {
          "@id": "schema:Text"
        },
        {
          "@id": "schema:URL"
        },
        {
          "@id": "schema:Boolean"
        },
        {
          "@id": "schema:StructuredValue"
        }
      ]
    },
    {
      "@id": "prov:wasAttributedTo",
      "schema:domainIncludes": {
        "@id": "reproschema:Response"
      },
      "schema:rangeIncludes": {
        "@id": "reproschema:Participant"
      }
    },
    {
      "@id": "reproschema:Response",
      "@type": [
        "rdfs:Class",
        "prov:Entity"
      ],
      "rdfs:comment": "Describes the response of an item.",
      "rdfs:label": "Response",
      "rdfs:subClassOf": {
        "@id": "schema:CreativeWork"
      }
    },
    {
      "@id": "reproschema:preamble",
      "@type": "rdf:Property",
      "schema:rangeIncludes": [
        {
          "@id": "schema:Text"
        },
        {
          "@id": "rdf:langString"
        }
      ],
      "rdfs:comment": "The preamble for an assessment",
      "rdfs:label": "Preamble"
    },
    {
      "@id": "reproschema:allow",
      "@type": "rdf:Property",
      "schema:rangeIncludes": {
        "@id": "schema:Thing"
      },
      "rdfs:comment": "An array of items indicating properties allowed on an activity or protocol ",
      "rdfs:label": "allow"
    },
    {
      "@id": "reproschema:limit",
      "@type": "rdf:Property",
      "schema:rangeIncludes": {
        "@id": "schema:Text"
      },
      "rdfs:comment": "An element to limit the duration (uses ISO 8601) this activity is allowed to be completed by once activity is available.",
      "rdfs:label": "limit"
    },
    {
      "@id": "reproschema:DisableBack",
      "@type": "rdfs:Class",
      "rdfs:comment": "Indicates (by boolean) if we can go back to a completed assessment in a protocol.",
      "rdfs:label": "Disable redo"
    },
    {
      "@id": "reproschema:AutoAdvance",
      "@type": "rdfs:Class",
      "rdfs:comment": "Indicates (by boolean) if assessments in a protocol can auto advance or not.",
      "rdfs:label": "Auto advance"
    },
    {
      "@id": "reproschema:TimedOut",
      "@type": "rdfs:Class",
      "rdfs:comment": "A boolean element to describe if the response did not occur within the prescribed time.",
      "rdfs:label": "Response timed out"
    },
    {
      "@id": "skos:prefLabel",
      "@type": "rdf:Property",
      "schema:domainIncludes": {
        "@id": "reproschema:Activity"
      },
      "schema:rangeIncludes": {
        "@id": "schema:Text"
      },
      "rdfs:comment": "The preferred label.",
      "rdfs:label": "preferred label"
    },
    {
      "@id": "schema:description",
      "schema:domainIncludes": {
        "@id": "reproschema:Activity"
      }
    },
    {
      "@id": "schema:schemaVersion",
      "schema:domainIncludes": {
        "@id": "reproschema:Activity"
      }
    },
    {
      "@id": "schema:version",
      "schema:domainIncludes": {
        "@id": "reproschema:Activity"
      }
    },
    {
      "@id": "schema:citation",
      "schema:domainIncludes": {
        "@id": "reproschema:Activity"
      }
    },
    {
      "@id": "reproschema:preamble",
      "schema:domainIncludes": {
        "@id": "reproschema:Activity"
      }
    },
    {
      "@id": "reproschema:order",
      "schema:domainIncludes": {
        "@id": "reproschema:Activity"
      }
    },
    {
      "@id": "reproschema:shuffle",
      "schema:domainIncludes": {
        "@id": "reproschema:Activity"
      }
    },
    {
      "@id": "reproschema:addProperties",
      "schema:domainIncludes": {
        "@id": "reproschema:Activity"
      }
    },
    {
      "@id": "reproschema:scoringLogic",
      "schema:domainIncludes": {
        "@id": "reproschema:Activity"
      }
    },
    {
      "@id": "schema:about",
      "schema:domainIncludes": {
        "@id": "reproschema:Activity"
      }
    },
    {
      "@id": "reproschema:Activity",
      "@type": [
        "rdfs:Class",
        "prov:Entity",
        "prov:Plan",
        "nidm:Assessment"
      ],
      "rdfs:comment": "An assessment in a protocol.",
      "rdfs:label": "Activity",
      "rdfs:subClassOf": {
        "@id": "schema:CreativeWork"
      }
    },
    {
      "@id": "nidm:subject_id",
      "schema:domainIncludes": {
        "@id": "reproschema:Participant"
      },
      "rdfs:comment": "The identifier of a participant",
      "rdfs:label": "Participant identifier"
    },
    {
      "@id": "reproschema:Participant",
      "@type": [
        "rdfs:Class",
        "prov:Person"
      ],
      "rdfs:comment": "An Agent describing characteristics associated with a participant.",
      "rdfs:label": "Participant",
      "rdfs:subClassOf": {
        "@id": "prov:Agent"
      }
    },
    {
      "@id": "reproschema:choices",
      "@type": "rdf:Property",
      "schema:rangeIncludes": [
        {
          "@id": "reproschema:Choice"
        },
        {
          "@id": "schema:URL"
        }
      ],
      "schema:sameAs": {
        "@id": "schema:itemListElement"
      },
      "rdfs:comment": "An array to list the available options for response of the Field item.",
      "rdfs:label": "choices"
    },
    {
      "@id": "reproschema:Skipped",
      "@type": "rdfs:Class",
      "rdfs:comment": "An element to describe the choice when the item is skipped.",
      "rdfs:label": "Skipped"
    },
    {
      "@id": "reproschema:source",
      "@type": "rdf:Property",
      "schema:rangeIncludes": {
        "@id": "rdf:langString"
      },
      "rdfs:comment": "An element to define the source (eg. RedCap, NDA) where the note was taken from.",
      "rdfs:label": "source"
    },
    {
      "@id": "reproschema:value",
      "@type": "rdf:Property",
      "schema:rangeIncludes": [
        {
          "@id": "schema:Boolean"
        },
        {
          "@id": "schema:StructuredValue"
        },
        {
          "@id": "schema:Number"
        },
        {
          "@id": "schema:Text"
        },
        {
          "@id": "schema:URL"
        }
      ],
      "schema:sameAs": {
        "@id": "schema:value"
      },
      "rdfs:comment": "The value for each option in choices or in additionalNotesObj",
      "rdfs:label": "value"
    },
    {
      "@id": "schema:version",
      "schema:domainIncludes": {
        "@id": "reproschema:SoftwareAgent"
      }
    },
    {
      "@id": "schema:url",
      "schema:domainIncludes": {
        "@id": "reproschema:SoftwareAgent"
      }
    },
    {
      "@id": "reproschema:SoftwareAgent",
      "@type": [
        "rdfs:Class",
        "prov:SoftwareAgent"
      ],
      "rdfs:comment": "Captures information about some action that took place. It also links to information (entities) that were used during the activity",
      "rdfs:label": "Software Agent"
    },
    {
      "@id": "reproschema:statusOptions",
      "@type": "rdf:Property",
      "schema:rangeIncludes": {
        "@id": "schema:Text"
      },
      "rdfs:comment": "Provides information on whether or not a field item wants to be accompanied by the additional status option(s) defined in \u201cstatusOptions\u201d",
      "rdfs:label": "Status options"
    },
    {
      "@id": "schema:image",
      "schema:domainIncludes": {
        "@id": "reproschema:Choice"
      }
    },
    {
      "@id": "schema:name",
      "schema:domainIncludes": {
        "@id": "reproschema:Choice"
      }
    },
    {
      "@id": "schema:value",
      "schema:domainIncludes": {
        "@id": "reproschema:Choice"
      },
      "schema:rangeIncludes": [
        {
          "@id": "reproschema:Skipped"
        },
        {
          "@id": "reproschema:DontKnow"
        }
      ]
    },
    {
      "@id": "reproschema:Choice",
      "@type": "rdfs:Class",
      "rdfs:comment": "An object to describe a response option.",
      "rdfs:label": "Response choice"
    },
    {
      "@id": "reproschema:column",
      "@type": "rdf:Property",
      "schema:rangeIncludes": {
        "@id": "rdf:langString"
      },
      "rdfs:comment": "An element to define the column name where the note was taken from.",
      "rdfs:label": "column"
    },
    {
      "@id": "skos:prefLabel",
      "@type": "rdf:Property",
      "schema:domainIncludes": {
        "@id": "reproschema:Protocol"
      },
      "schema:rangeIncludes": {
        "@id": "schema:Text"
      },
      "rdfs:comment": "The preferred label.",
      "rdfs:label": "preferred label"
    },
    {
      "@id": "schema:description",
      "schema:domainIncludes": {
        "@id": "reproschema:Protocol"
      }
    },
    {
      "@id": "schema:schemaVersion",
      "schema:domainIncludes": {
        "@id": "reproschema:Protocol"
      }
    },
    {
      "@id": "schema:version",
      "schema:domainIncludes": {
        "@id": "reproschema:Protocol"
      }
    },
    {
      "@id": "reproschema:order",
      "schema:domainIncludes": {
        "@id": "reproschema:Protocol"
      }
    },
    {
      "@id": "reproschema:shuffle",
      "schema:domainIncludes": {
        "@id": "reproschema:Protocol"
      }
    },
    {
      "@id": "reproschema:addProperties",
      "schema:domainIncludes": {
        "@id": "reproschema:Protocol"
      }
    },
    {
      "@id": "reproschema:allow",
      "schema:domainIncludes": {
        "@id": "reproschema:Protocol"
      }
    },
    {
      "@id": "reproschema:landingPage",
      "schema:domainIncludes": {
        "@id": "reproschema:Protocol"
      }
    },
    {
      "@id": "reproschema:scoringLogic",
      "schema:domainIncludes": {
        "@id": "reproschema:Protocol"
      }
    },
    {
      "@id": "schema:about",
      "schema:domainIncludes": {
        "@id": "reproschema:Protocol"
      }
    },
    {
      "@id": "reproschema:Protocol",
      "@type": [
        "rdfs:Class",
        "prov:Plan",
        "prov:Entity"
      ],
      "rdfs:comment": "A representation of a study which comprises one or more assessments.",
      "rdfs:label": "Protocol",
      "rdfs:subClassOf": {
        "@id": "schema:CreativeWork"
      }
    },
    {
      "@id": "skos:prefLabel",
      "@type": "rdf:Property",
      "schema:domainIncludes": {
        "@id": "reproschema:Field"
      },
      "schema:rangeIncludes": {
        "@id": "schema:Text"
      },
      "rdfs:comment": "The preferred label.",
      "rdfs:label": "preferred label"
    },
    {
      "@id": "schema:description",
      "schema:domainIncludes": {
        "@id": "reproschema:Field"
      }
    },
    {
      "@id": "schema:schemaVersion",
      "schema:domainIncludes": {
        "@id": "reproschema:Field"
      }
    },
    {
      "@id": "schema:version",
      "schema:domainIncludes": {
        "@id": "reproschema:Field"
      }
    },
    {
      "@id": "reproschema:preamble",
      "schema:domainIncludes": {
        "@id": "reproschema:Field"
      }
    },
    {
      "@id": "schema:question",
      "schema:domainIncludes": {
        "@id": "reproschema:Field"
      }
    },
    {
      "@id": "schema:image",
      "@type": "rdf:Property",
      "schema:domainIncludes": {
        "@id": "reproschema:Field"
      },
      "rdfs:comment": "An image of the item. This can be a <a class=\"localLink\" href=\"http://schema.org/URL\">URL</a> or a fully described <a class=\"localLink\" href=\"http://schema.org/ImageObject\">ImageObject</a>.",
      "rdfs:label": "image"
    },
    {
      "@id": "reproschema:inputType",
      "schema:domainIncludes": {
        "@id": "reproschema:Field"
      }
    },
    {
      "@id": "schema:readonlyValue",
      "schema:domainIncludes": {
        "@id": "reproschema:Field"
      }
    },
    {
      "@id": "schema:isPartOf",
      "schema:domainIncludes": {
        "@id": "reproschema:Field"
      },
      "schema:rangeIncludes": {
        "@id": "reproschema:Activity"
      }
    },
    {
      "@id": "reproschema:responseOptions",
      "schema:domainIncludes": {
        "@id": "reproschema:Field"
      }
    },
    {
      "@id": "schema:associatedMedia",
      "schema:domainIncludes": {
        "@id": "reproschema:Field"
      }
    },
    {
      "@id": "schema:about",
      "schema:domainIncludes": {
        "@id": "reproschema:Field"
      }
    },
    {
      "@id": "reproschema:Field",
      "@type": [
        "rdfs:Class",
        "prov:Entity",
        "nidm:DataElement"
      ],
      "rdfs:comment": "An item in an assessment.",
      "rdfs:label": "Field",
      "rdfs:subClassOf": {
        "@id": "schema:CreativeWork"
      }
    },
    {
      "@id": "prov:used",
      "schema:domainIncludes": {
        "@id": "reproschema:ResponseActivity"
      }
    },
    {
      "@id": "schema:inLanguage",
      "schema:domainIncludes": {
        "@id": "reproschema:ResponseActivity"
      }
    },
    {
      "@id": "prov:startedAtTime",
      "schema:domainIncludes": {
        "@id": "reproschema:ResponseActivity"
      }
    },
    {
      "@id": "prov:endedAtTime",
      "schema:domainIncludes": {
        "@id": "reproschema:ResponseActivity"
      }
    },
    {
      "@id": "prov:endedAtTime",
      "schema:domainIncludes": {
        "@id": "reproschema:ResponseActivity"
      }
    },
    {
      "@id": "prov:generated",
      "schema:domainIncludes": {
        "@id": "reproschema:ResponseActivity"
      }
    },
    {
      "@id": "reproschema:ResponseActivity",
      "@type": [
        "rdfs:Class",
        "prov:Activity"
      ],
      "rdfs:comment": "Captures information about some action that took place. It also links to information (entities) that were used during the activity",
      "rdfs:label": "ResponseActivity",
      "rdfs:subClassOf": {
        "@id": "schema:CreativeWork"
      }
    },
    {
      "@id": "reproschema:valueType",
      "schema:domainIncludes": {
        "@id": "reproschema:ResponseOption"
      }
    },
    {
      "@id": "schema:minValue",
      "schema:domainIncludes": {
        "@id": "reproschema:ResponseOption"
      }
    },
    {
      "@id": "schema:maxValue",
      "schema:domainIncludes": {
        "@id": "reproschema:ResponseOption"
      }
    },
    {
      "@id": "reproschema:multipleChoice",
      "schema:domainIncludes": {
        "@id": "reproschema:ResponseOption"
      }
    },
    {
      "@id": "reproschema:datumType",
      "schema:domainIncludes": {
        "@id": "reproschema:ResponseOption"
      }
    },
    {
      "@id": "schema:unitCode",
      "schema:domainIncludes": {
        "@id": "reproschema:ResponseOption"
      }
    },
    {
      "@id": "reproschema:choices",
      "schema:domainIncludes": {
        "@id": "reproschema:ResponseOption"
      }
    },
    {
      "@id": "reproschema:ResponseOption",
      "@type": "rdfs:Class",
      "rdfs:comment": "An element (object or by URL)to describe the properties of response of the Field item.",
      "rdfs:label": "Response option"
    },
    {
      "@id": "reproschema:variableName",
      "@type": "rdf:Property",
      "schema:rangeIncludes": {
        "@id": "schema:Text"
      },
      "rdfs:comment": "The name used to represent an item.",
      "rdfs:label": "variableName"
    },
    {
      "@id": "reproschema:isAbout",
      "@type": "rdf:Property",
      "schema:rangeIncludes": [
        {
          "@id": "reproschema:Activity"
        },
        {
          "@id": "reproschema:Field"
        }
      ],
      "rdfs:comment": "A pointer to the node describing the item.",
      "rdfs:label": "isAbout"
    },
    {
      "@id": "reproschema:variableName",
      "@type": "rdf:Property",
      "schema:domainIncludes": {
        "@id": "reproschema:ComputeSpecification"
      },
      "rdfs:comment": "The name used to represent an item.",
      "rdfs:label": "variableName"
    },
    {
      "@id": "reproschema:jsExpression",
      "@type": "rdf:Property",
      "schema:domainIncludes": {
        "@id": "reproschema:ComputeSpecification"
      },
      "rdfs:comment": "A JavaScript expression for computations.",
      "rdfs:label": "JavaScript Expression"
    },
    {
      "@id": "reproschema:ComputeSpecification",
      "@type": "rdfs:Class",
      "rdfs:comment": "An object to define computations in an activity or protocol.",
      "rdfs:label": "Compute Specification"
    },
    {
      "@id": "reproschema:addProperties",
      "@type": "rdf:Property",
      "schema:rangeIncludes": {
        "@id": "reproschema:AdditionalProperty"
      },
      "rdfs:comment": "An array of objects to describe the various properties added to assessments and fields.",
      "rdfs:label": "addProperties"
    },
    {
      "@id": "reproschema:compute",
      "@type": "rdf:Property",
      "schema:rangeIncludes": {
        "@id": "reproschema:ComputeSpecification"
      },
      "rdfs:comment": "An array of objects indicating computations in an activity or protocol and maps it to the corresponding Field item. scoring logic is a subset of all computations that could be performed and not all computations will be scoring. For example, one may want to do conversion from one unit to another. ",
      "rdfs:label": "computation"
    },
    {
      "@id": "reproschema:datumType",
      "@type": "rdf:Property",
      "schema:rangeIncludes": [
        {
          "@id": "schema:URL"
        },
        {
          "@id": "schema:Text"
        }
      ],
      "rdfs:comment": "Indicates what type of datum the response is (e.g. range,count,scalar etc.) for the Field item.",
      "rdfs:label": "datumType"
    },
    {
      "@id": "reproschema:additionalNotesObj",
      "@type": "rdf:Property",
      "schema:rangeIncludes": {
        "@id": "reproschema:AdditionalNoteObj"
      },
      "rdfs:comment": "A set of objects to define notes in a field. For example, most Redcap and NDA data dictionaries have notes for each item which needs to be captured in reproschema.",
      "rdfs:label": "additional notes"
    },
    {
      "@id": "reproschema:valueType",
      "@type": "rdf:Property",
      "schema:rangeIncludes": [
        {
          "@id": "schema:Text"
        },
        {
          "@id": "rdf:langString"
        }
      ],
      "rdfs:comment": "The type of the response of an item. For example, string, integer, etc.",
      "rdfs:label": "The type of the response"
    },
    {
      "@id": "reproschema:isVis",
      "@type": "rdf:Property",
      "schema:rangeIncludes": [
        {
          "@id": "schema:Boolean"
        },
        {
          "@id": "schema:Text"
        }
      ],
      "rdfs:comment": "An element to describe (by boolean or conditional statement) visibility conditions of items in an assessment.",
      "rdfs:label": "visibility"
    },
    {
      "@id": "reproschema:responseOptions",
      "@type": "rdf:Property",
      "schema:rangeIncludes": [
        {
          "@id": "reproschema:ResponseOption"
        },
        {
          "@id": "schema:URL"
        }
      ],
      "rdfs:comment": "An element (object or by URL)to describe the properties of response of the Field item.",
      "rdfs:label": "Response options"
    },
    {
      "@id": "reproschema:source",
      "schema:domainIncludes": {
        "@id": "reproschema:AdditionalNoteObj"
      }
    },
    {
      "@id": "reproschema:column",
      "schema:domainIncludes": {
        "@id": "reproschema:AdditionalNoteObj"
      }
    },
    {
      "@id": "reproschema:value",
      "schema:domainIncludes": {
        "@id": "reproschema:AdditionalNoteObj"
      }
    },
    {
      "@id": "reproschema:AdditionalNoteObj",
      "@type": "rdfs:Class",
      "rdfs:comment": "A set of objects to define notes in a field. For example, most Redcap and NDA data dictionaries have notes for each item which needs to be captured in reproschema",
      "rdfs:label": "Additional Notes Object"
    },
    {
      "@id": "reproschema:randomMaxDelay",
      "@type": "rdf:Property",
      "schema:rangeIncludes": {
        "@id": "schema:Text"
      },
      "rdfs:comment": "Present activity/item within some random offset of activity available time up to the maximum specified by this ISO 8601 duration",
      "rdfs:label": "randomMaxDelay"
    },
    {
      "@id": "reproschema:landingPage",
      "@type": "rdf:Property",
      "schema:rangeIncludes": [
        {
          "@id": "schema:URL"
        },
        {
          "@id": "schema:Text"
        }
      ],
      "rdfs:comment": "An element (by URL) to point to the protocol readme or landing page.",
      "rdfs:label": "Landing page content"
    },
    {
      "@id": "reproschema:variableName",
      "schema:domainIncludes": {
        "@id": "reproschema:AdditionalProperty"
      }
    },
    {
      "@id": "reproschema:isAbout",
      "schema:domainIncludes": {
        "@id": "reproschema:AdditionalProperty"
      }
    },
    {
      "@id": "schema:valueRequired",
      "schema:domainIncludes": {
        "@id": "reproschema:AdditionalProperty"
      }
    },
    {
      "@id": "skos:prefLabel",
      "@type": "rdf:Property",
      "schema:domainIncludes": {
        "@id": "reproschema:AdditionalProperty"
      },
      "rdfs:comment": "The preferred label.",
      "rdfs:label": "preferred label"
    },
    {
      "@id": "reproschema:isVis",
      "schema:domainIncludes": {
        "@id": "reproschema:AdditionalProperty"
      }
    },
    {
      "@id": "reproschema:randomMaxDelay",
      "@type": "rdf:Property",
      "schema:domainIncludes": {
        "@id": "reproschema:AdditionalProperty"
      }
    },
    {
      "@id": "reproschema:schedule",
      "@type": "rdf:Property",
      "schema:domainIncludes": {
        "@id": "reproschema:AdditionalProperty"
      }
    },
    {
      "@id": "reproschema:limit",
      "@type": "rdf:Property",
      "schema:domainIncludes": {
        "@id": "reproschema:AdditionalProperty"
      }
    },
    {
      "@id": "reproschema:maxRetakes",
      "@type": "rdf:Property",
      "schema:domainIncludes": {
        "@id": "reproschema:AdditionalProperty"
      }
    },
    {
      "@id": "reproschema:AdditionalProperty",
      "@type": "rdfs:Class",
      "rdfs:comment": "An object to describe the various properties added to assessments and fields.",
      "rdfs:label": "Additional properties"
    },
    {
      "@id": "reproschema:jsExpression",
      "@type": "rdf:Property",
      "schema:rangeIncludes": [
        {
          "@id": "schema:Text"
        },
        {
          "@id": "schema:Boolean"
        }
      ],
      "rdfs:comment": "A JavaScript expression to compute a score from other variables.",
      "rdfs:label": "JavaScript Expression"
    }
  ]
}
